Recorded defviews in Snapshot

LSPLogAnalyzer/MyParser.lean
@@ -1,5 +1,5 @@
 import Lean
-import LSPLogAnalyzer
+import LSPLogAnalyzer.Definitions
 
 open Lean
 open Parser
@@ -7,41 +7,19 @@ open Parser.Command
 open Elab
 open Elab.Command
 open System
-open LSPLogAnalyzer
 
 open Std
 
-namespace Lean.Elab.DefView
 
-  def getLspRange (dv : DefView) (inCtx : InputContext) : Option Lsp.Range :=
-    dv.ref.getRange?.map inCtx.fileMap.utf8RangeToLspRange
-
-  def getId (dv : DefView) : Name :=
-    match dv.declId.find? (·.isIdent) with
-    | none => .anonymous
-    | some id => id.getId
-
-  instance : ToString DefKind where
-    toString
-    | .theorem => "theorem"
-    | .abbrev => "abbrev"
-    | .opaque => "opaque"
-    | .example => "example"
-    | .instance => "instance"
-    | .def => "def"
-
-  instance : ToString DefView where
-    toString | dv@{ kind, .. } => s!"{kind} {dv.getId}"
-
-end Lean.Elab.DefView
+namespace LSPLogAnalyzer
 
 def collectDefLikes (fname : FilePath) (contents : String)
-    : CommandElabM (Array (DefView × Option Lsp.Range)) := do
-  let env ← getEnv -- FIXME : write mkFreshEnv
+    : CommandElabM (Array Definition) := do
+  let env ← getEnv
   let inCtx := mkInputContext contents fname.toString
   let pmCtx := { env, options := {} }
   let (headerStx, mps, msgl) ← parseHeader inCtx
-  -- TODO : elab the header, not forgetting to update env
+  -- TODO : elab the header? (not forgetting to update env)
 
   let mut mps := mps
   let mut msgl := msgl
@@ -52,31 +30,25 @@ def collectDefLikes (fname : FilePath) (contents : String)
     (cmdStx, mps, msgl) := parseCommand inCtx pmCtx mps msgl
     -- let _ ← elabCommand cmdStx  -- TODO : necessary ?
     if cmdStx.getNumArgs > 1 && isDefLike cmdStx[1] then
-      let defView ← mkDefView {} cmdStx[1]
-      res := res.push (defView, defView.getLspRange inCtx)
+      let defview ← mkDefView {} cmdStx[1]
+      let name := defview.getId
+      let range := defview.getLspRange inCtx
+      res := res.push { name, defview, range }
   until isTerminalCommand cmdStx
 
   return res
 
-#eval show Elab.Command.CommandElabM _ from do
-  let fname := "/home/ameyer/Nextcloud/Eiffel/Code/lean4/lsp_log_analyzer/Example.lean"
-  let contents :=
-"import Lean
+def runCollectDefLikes (fname : FilePath) (contents : String)
+    : IO (Array Definition) := do
+  let action := collectDefLikes fname contents
+  let ctx := {
+    fileName := fname.toString,
+    fileMap := FileMap.ofString contents,
+    snap? := none,
+    cancelTk? := none }
+  let env ← mkEmptyEnvironment
+  let s := { env := env, maxRecDepth := 10 }
+  action.run ctx |>.run' s |>.toIO
+    fun _ => IO.Error.mkOtherError 0 "dunno"
 
-variable {p q r : Prop}
-
-theorem imp_trans (hpq : p → q) (hqr : q → r) : p → r := by
-  intro hp
-  exact hqr (hpq hp)
-
-theorem or_comm' (h : p ∨ q) : q ∨ p := by
-  rcases h with h | h
-  right
-  exact h
-  left
-  exact h
-"
-  let defs ← collectDefLikes fname contents
-  defs.forM (fun
-  | (dv, .some r) => IO.println s!"{dv} {r}"
-  | (dv, .none) => IO.println s!"{dv} (no position)")
+end LSPLogAnalyzer
