LSPLogAnalyzer.lean
@@ -1,3 +1,4 @@
 import LSPLogAnalyzer.Basic
-import LSPLogAnalyzer.FileState
+-- import LSPLogAnalyzer.FileState
 import LSPLogAnalyzer.PrettyGoals
+import LSPLogAnalyzer.MyParser
