LSPLogAnalyzer/Definitions.lean
@@ -1,0 +1,187 @@
+import Lean
+
+open Std.Time
+open Lean.Json
+open Lean.ToJson
+open Lean.FromJson
+open Lean.JsonRpc
+open Lean.Lsp
+open Lean.Elab
+
+
+abbrev Uri := String
+
+instance : Lean.ToJson ZonedDateTime where
+  toJson dt := dt.toISO8601String
+
+instance : Lean.FromJson ZonedDateTime where
+  fromJson?
+    | .str s => ZonedDateTime.fromISO8601String s
+    | _ => throw "Expected string when converting JSON to ZonedDateTime"
+
+/-- LSP log entry (new format). -/
+structure LogEntry where
+  time : ZonedDateTime
+  direction : MessageDirection
+  kind : MessageKind
+  msg : Message
+  deriving Lean.FromJson, Lean.ToJson
+
+instance : ToString LogEntry where
+  toString le := pretty $ toJson le
+
+instance : ToString MessageDirection where
+  toString
+  | .serverToClient => "server→client"
+  | .clientToServer => "client→server"
+
+instance : Coe LogEntry Message := ⟨LogEntry.msg⟩
+
+
+/-- File change event. -/
+structure ChangeEvent where
+  time : ZonedDateTime
+  version : Nat
+  changes : Array TextDocumentContentChangeEvent
+
+instance : ToString Range where
+  toString | ⟨⟨sl, sc⟩, ⟨el, ec⟩⟩ => s!"[{sl}:{sc}, {el}:{ec}]"
+
+instance : ToString TextDocumentContentChangeEvent where
+  toString ev := match ev with
+  | .fullChange _ => "full text"
+  | .rangeChange range text => s!"\"{text}\" at {range}"
+
+instance : ToString ChangeEvent where
+  toString ev :=
+    let ranges := ev.changes.map toString
+    s!"[{ev.time} - version {ev.version}] " ++ ", ".intercalate ranges.toList
+
+
+namespace Lean.Elab.DefView
+
+  def getLspRange (dv : DefView) (inCtx : Parser.InputContext) : Lsp.Range :=
+    let range := dv.ref.getRange?.get!
+    inCtx.fileMap.utf8RangeToLspRange range
+
+  def getId (dv : DefView) : Name :=
+    match dv.declId.find? (·.isIdent) with
+    | none => .anonymous
+    | some id => id.getId
+
+  instance : ToString DefKind where
+    toString
+    | .theorem => "theorem"
+    | .abbrev => "abbrev"
+    | .opaque => "opaque"
+    | .example => "example"
+    | .instance => "instance"
+    | .def => "def"
+
+  instance : ToString DefView where
+    toString | dv@{ kind, .. } => s!"{kind} {dv.getId}"
+
+end Lean.Elab.DefView
+
+/-- File snapshot. -/
+structure Definition where
+  name : Lean.Name
+  range : Range
+  defview : DefView
+  diags : Array Diagnostic := #[]
+
+instance : ToString Definition where
+  toString
+  | { name, range, defview, .. } => s!"{defview.kind} {range} {name}"
+
+
+/-- File snapshot. -/
+structure Snapshot where
+  time : ZonedDateTime
+  doc : TextDocumentItem
+  goals : Array Lean.Widget.InteractiveGoal  -- not used yet
+  diags : Array Diagnostic
+  deflikes : Array Definition
+
+instance : ToString DiagnosticSeverity where
+  toString
+  | .information => "info"
+  | .error => "error"
+  | .warning => "warning"
+  | .hint => "hint"
+
+instance : ToString Diagnostic where
+  toString diag :=
+    let s := match diag.severity? with
+    | some s => s!" ({s})"
+    | none => ""
+    s!"{diag.range}{s} {diag.message}"
+
+instance : ToString Snapshot where
+  toString snap :=
+    let v := snap.doc.version
+    let diags := match snap.diags with
+    | #[] => ""
+    | _ => s!"[diagnostics]\n{String.intercalate "\n" $ snap.diags.toList.map toString}\n"
+    let deflikes := match snap.deflikes with
+    | #[] => ""
+    | _ => s!"[definitions]\n{String.intercalate "\n" $ snap.deflikes.toList.map toString}\n"
+    s!"[begin version {v} ({snap.time})]\n\
+      {snap.doc.text.trim}\n\
+      {diags}\
+      {deflikes}\
+      [end version {v}]"
+
+
+/-- Per-file replay state. -/
+structure FileState where
+  snapshots : Array Snapshot := #[]
+  changes : Array ChangeEvent := #[]
+  currentSnap : Option Snapshot := none   -- not used yet
+  currentDiags : Array Diagnostic := #[]  -- not used yet
+deriving Inhabited
+
+instance : ToString FileState where
+  toString fs :=
+    let ssnaps := String.intercalate "\n\n" $ fs.snapshots.toList.map toString
+    let schanges := match fs.changes with
+    | #[] => ""
+    | _ => "Pending changes:\n" ++ (String.intercalate "\n" $ fs.changes.toList.map toString)
+    s!"Recorded snapshots:\n{ssnaps}\n\n\
+       {schanges}"
+
+/-- Log entry tracking error. -/
+structure TrackingError where
+  message : String
+  -- entry : LogEntry
+
+instance : ToString TrackingError where
+  toString te := te.message
+
+
+/-- Global tracker. -/
+structure Tracker where
+  files : Std.TreeMap Uri FileState Ord.compare := {}
+  errors : Array TrackingError := #[]
+  line : Nat := 1
+  requests : Std.TreeMap RequestID (Request Lean.Json) := {}
+deriving Inhabited
+
+instance : ToString Tracker where
+  toString tracker :=
+    let fss := "\n\n".intercalate $ tracker.files.toList.map
+      fun (uri, fs) => s!"State for {uri}:\n\n{fs}"
+    let errors := "\n".intercalate $ tracker.errors.toList.map toString
+    let requests := "\n".intercalate $ tracker.requests.toList.map
+      fun (id, req) =>
+        let m := match req.method with
+        | "$/lean/rpc/call" =>
+            match fromJson? req.param with
+            | .ok (param : RpcCallParams) => s!"{req.method} ({param.method})"
+            | _ => req.method
+        | _ => req.method
+        s!"{id}:\t{m}"
+    s!"{fss}\n\nErrors:\n{errors}\n\nPending requests:\n{requests}"
+
+/-- Tracker monad. -/
+abbrev TrackerM := StateT Tracker IO
